Qed LockedStack proof

new/proof/github_com/goose_lang/goose/testdata/examples/elimination_stack.v
@@ -22,24 +22,25 @@ Context `{!globalsGS Σ} {go_ctx : GoContext}.
 
 Context `{!locked_stackG Σ}.
 
-Definition own_locked_stack γ (σ : list go_string) : iProp Σ :=
+Definition own_LockedStack γ (σ : list go_string) : iProp Σ :=
   ghost_var γ (1/2) σ.
-#[global] Opaque own_locked_stack.
-#[local] Transparent own_locked_stack.
+#[global] Opaque own_LockedStack.
+#[local] Transparent own_LockedStack.
 
 Definition is_LockedStack s γ : iProp Σ :=
   "#Hmu" ∷ (is_Mutex (struct.field_ref_f chan_spec_raw_examples.LockedStack "mu" s)
               (∃ stack_sl (stack : list go_string),
                   "stack" ∷ s ↦s[chan_spec_raw_examples.LockedStack :: "stack"] stack_sl ∗
-                  "Hstack_sl" ∷ stack_sl ↦* stack ∗
-                  "Hstack_cap" ∷ own_slice_cap go_string stack_sl (DfracOwn 1) ∗
-                  "Hstack_auth" ∷ ghost_var γ (1/2) stack
-    )).
+                  "Hsl" ∷ stack_sl ↦* stack ∗
+                  "Hcap" ∷ own_slice_cap go_string stack_sl (DfracOwn 1) ∗
+                  "Hauth" ∷ ghost_var γ (1/2) (reverse stack)
+    )) ∗
+  "_" ∷ True.
 
 Lemma wp_NewLockedStack :
   {{{ is_pkg_init chan_spec_raw_examples }}}
     @! chan_spec_raw_examples.NewLockedStack #()
-  {{{ s γ, RET #s; is_LockedStack s γ ∗ own_locked_stack γ [] }}}.
+  {{{ s γ, RET #s; is_LockedStack s γ ∗ own_LockedStack γ [] }}}.
 Proof.
   wp_start. unshelve wp_apply wp_slice_make2; try tc_solve; first word.
   iIntros (stack_sl) "[stack_sl cap]". rewrite replicate_0.
@@ -48,6 +49,80 @@ Proof.
   iMod (ghost_var_alloc []) as (γ) "[Hstack_auth Hstack_frag]".
   iApply "HΦ". iDestruct (struct_fields_split with "Hs") as "H". iNamed "H".
   simpl. iMod (init_Mutex with "[$] [-Hstack_frag]") as "$"; by iFrame.
+Qed.
+
+Lemma wp_LockedStack__Push v γ s :
+  ∀ Φ,
+  is_pkg_init chan_spec_raw_examples ∗ is_LockedStack s γ -∗
+  (|={⊤,∅}=> ∃ σ, own_LockedStack γ σ ∗ (own_LockedStack γ (v :: σ) ={∅,⊤}=∗ Φ #())) -∗
+  WP s @ (ptrT.id chan_spec_raw_examples.LockedStack.id) @ "Push" #v {{ Φ }}.
+Proof.
+  wp_start as "#His". wp_auto. iNamed "His".
+  wp_apply (wp_Mutex__Lock with "[$Hmu]"). iIntros "[Hlocked Hi]".
+  iNamedSuffix "Hi" "_inv". wp_auto.
+  wp_apply wp_slice_literal. iIntros "% Htmp". wp_auto.
+  wp_apply (wp_slice_append with "[$Hsl_inv $Hcap_inv $Htmp]").
+  iIntros (stack_sl') "(Hsl_inv & Hcap_inv & _)". wp_auto.
+  iApply fupd_wp. iMod "HΦ" as "(% & Hl & HΦ)". iCombine "Hl Hauth_inv" gives %[_ ->].
+  iMod (ghost_var_update_2 with "Hl Hauth_inv") as "[Hl Hauth_inv]".
+  { compute_done. }
+  iMod ("HΦ" with "Hl") as "HΦ". iModIntro.
+  iCombineNamed "*_inv" as "Hi".
+  wp_apply (wp_Mutex__Unlock with "[$Hmu $Hlocked Hi]").
+  { iNamed "Hi". iFrame. rewrite reverse_app. iFrame. }
+  iFrame.
+Qed.
+
+Lemma wp_LockedStack__Pop γ s :
+  ∀ Φ,
+  is_pkg_init chan_spec_raw_examples ∗ is_LockedStack s γ -∗
+  (|={⊤,∅}=> ∃ σ, own_LockedStack γ σ ∗
+                 (match σ with
+                  | [] => own_LockedStack γ [] ={∅,⊤}=∗ Φ (#"", #false)%V
+                  | v :: σ => own_LockedStack γ σ ={∅,⊤}=∗ Φ (#v, #true)%V
+                  end)
+  ) -∗
+  WP s @ (ptrT.id chan_spec_raw_examples.LockedStack.id) @ "Pop" #() {{ Φ }}.
+Proof.
+  wp_start as "#His". wp_auto. iNamed "His".
+  wp_apply (wp_Mutex__Lock with "[$Hmu]"). iIntros "[Hlocked Hi]".
+  iNamedSuffix "Hi" "_inv". wp_auto.
+  iDestruct (own_slice_len with "[$]") as %Hlen.
+  iDestruct (own_slice_cap_wf with "[$]") as %Hcap.
+  iApply fupd_wp. iMod "HΦ" as "(% & Hl & HΦ)".
+  iCombine "Hl Hauth_inv" gives %[_ Heq].
+  apply (f_equal reverse) in Heq. rewrite reverse_involutive in Heq.
+  subst. destruct σ; simpl in *.
+  - iMod ("HΦ" with "Hl") as "HΦ".
+    iModIntro. rewrite bool_decide_true.
+    2:{ revert Hlen; by len. }
+    wp_auto. iCombineNamed "*_inv" as "Hi".
+    wp_apply (wp_Mutex__Unlock with "[$Hmu $Hlocked Hi]").
+    { iNamed "Hi". iFrame. }
+    iFrame.
+  - iMod (ghost_var_update_2 with "Hl Hauth_inv") as "[Hl Hauth_inv]".
+    { compute_done. }
+    iMod ("HΦ" with "Hl") as "HΦ". iModIntro.
+    rewrite bool_decide_false; last (revert Hlen; by len).
+    wp_auto. wp_pure; first (revert Hlen; by len).
+    rewrite reverse_cons.
+    wp_apply (wp_load_slice_elem with "[$Hsl_inv]") as "Hsl_inv".
+    { revert Hlen; by len. }
+    { iPureIntro. rewrite lookup_app_r; last (revert Hlen; by len).
+      replace (_) with O by (revert Hlen; by len). done. }
+    (* NOTE: there are too many choices here... would be better to have at least
+       one "canonical" proof approach. *)
+    wp_apply (wp_slice_slice_with_cap with "[$Hsl_inv $Hcap_inv]").
+    { iPureIntro. revert Hlen Hcap; by len. }
+    iIntros "(_ & Hsl_inv & Hcap_inv)".
+    wp_auto.
+    iCombineNamed "*_inv" as "Hi".
+    wp_apply (wp_Mutex__Unlock with "[$Hmu $Hlocked Hi]").
+    { iNamed "Hi". iFrame. rewrite /subslice.
+      rewrite take_app_le; last (revert Hlen Hcap; by len).
+      rewrite take_ge; last (revert Hlen Hcap; by len).
+      rewrite drop_0 reverse_involutive. iFrame. }
+    iFrame.
 Qed.
 
 End locked_stack_proof.
